src/Iris/Algebra/BigOp.lean
@@ -1,0 +1,32 @@
+/-
+Copyright (c) 2026 Zongyuan Liu. All rights reserved.
+Released under Apache 2.0 license as described in the file LICENSE.
+Authors: Zongyuan Liu
+-/
+import Iris.Algebra.Monoid
+import Iris.Std.List
+import Iris.Std.PartialMap
+import Iris.Std.GenSets
+
+namespace Iris.Algebra
+
+/-! # Big Operators
+
+This file defines big operators (fold operations) at the abstract OFE level.
+These are parameterized by a monoid operation and include theorems about their properties.
+-/
+
+open OFE
+open Iris.Std
+
+def bigOpS {A : Type _} [DecidableEq A] {S : Type _} [OFE M] (op : M → M → M) {unit : M}
+  [MonoidOps op unit] (Φ : A → M) [LawfulFiniteSet S A] (m : S) : M :=
+  Set.fold (fun acc x => op acc (Φ x)) (by intro S' x y; simp only; rw [<-MonoidOps.op_comm]) unit m
+
+/-- Big op over set without index: `[^ op set] x ∈ l, P` -/
+scoped syntax atomic("[^") term " set]" ident " ∈ " term ", " term : term
+
+scoped macro_rules
+  | `([^ $o set] $x ∈ $l, $P) => `(bigOpS $o (fun _ $x => $P) $l)
+
+end Iris.Algebra
